erasure/theories/EAstUtils.v
@@ -267,6 +267,8 @@ Fixpoint string_of_term (t : term) : string :=
             ^ string_of_term c ^ ")"
   | tFix l n => "Fix(" ^ (string_of_list (string_of_def string_of_term) l) ^ "," ^ string_of_nat n ^ ")"
   | tCoFix l n => "CoFix(" ^ (string_of_list (string_of_def string_of_term) l) ^ "," ^ string_of_nat n ^ ")"
+  | tInt i => "Int(" ^ string_of_Z (proj1_sig i) ^ ")"
+  | tFloat f => "Float(" ^ "<float>" ^ ")"
   end.
 
 (** Compute all the global environment dependencies of the term *)
