safechecker/theories/PCUICSafeReduce.v
@@ -1256,6 +1256,8 @@ Section Reduce.
       unfold is_true in typ.
       unfold PCUICAst.fst_ctx in *.
       congruence.
+    - now eapply inversion_Int in typ.
+    - now eapply inversion_Float in typ.
   Qed.
   
   Definition isCoFix_app t :=
@@ -1287,6 +1289,8 @@ Section Reduce.
     - exfalso; eapply invert_fix_ind; eauto.
     - unfold isCoFix_app in cof.
       now rewrite decompose_app_mkApps in cof.
+    - now eapply inversion_Int in typ.
+    - now eapply inversion_Float in typ.
   Qed.
   
   Lemma whnf_fix_arg_whne mfix idx body Γ t before args aftr ty :
@@ -1435,6 +1439,11 @@ Section Reduce.
           apply inversion_App in h as (?&?&?&?&?); auto.
           apply inversion_Prod in t0 as (?&?&?&?&?); auto.
           eapply PCUICConversion.cumul_Sort_Prod_inv; eauto.
+      + exfalso.
+        eapply welltyped_context in h as [s Hs]; tas.
+        now eapply inversion_Int in Hs.
+      + exfalso; eapply welltyped_context in h as [s Hs]; tas.
+        now eapply inversion_Float in Hs.
     - unfold zipp. case_eq (decompose_stack π0). intros l ρ e.
       constructor. constructor. eapply whne_mkApps.
       eapply whne_rel_nozeta. assumption.
