template-coq/update_plugin.sh
@@ -4,7 +4,7 @@ TOCOPY="ast_denoter.ml ast_quoter.ml denoter.ml plugin_core.ml plugin_core.mli r
 
 # Test is gen-src is older than src
 if [[ "gen-src" -ot "src" || ! -f "gen-src/denoter.ml" || ! -f "gen-src/metacoq_template_plugin.cmxs" ||
-  "gen-src/extractable.ml" -nt "gen-src/metacoq_template_plugin.cmxs" ]]
+  "gen-src/extractable.ml" -nt "gen-src/metacoq_template_plugin.cmxs" || "$1" = "force" ]]
 then
     echo "Updating gen-src from src"
     mkdir -p build
@@ -12,9 +12,10 @@ then
     for x in ${TOCOPY}; do rm -f gen-src/$x; cp src/$x gen-src/$x; done
     echo "Renaming files to camelCase"
     (cd gen-src; ./to-lower.sh)
-    rm -f gen-src/*.d
+    rm -f gen-src/*.d gen-src/*.cm*
     # Fix an extraction bug: wrong type annotation on eq_equivalence
     patch -N -p0 < extraction.patch
+    patch -N -p0 < specFloat.patch
     exit 0
 else
     echo "Extracted code is up-to-date"
